\documentclass[11pt]{article}
\usepackage[T1]{fontenc}
\usepackage{beramono}
\usepackage{listings}
\usepackage[usenames,dvipsnames]{xcolor}
\usepackage[mathletters]{ucs}
\usepackage[utf8x]{inputenc}

\usepackage{mathtools}
\usepackage{geometry}
\usepackage{siunitx}
\usepackage{float}
\usepackage{graphicx}
\usepackage{xcolor}
\usepackage{tikz}
\usetikzlibrary{patterns}
\geometry{margin=2in,top=1in,bottom=1in}

\newcommand{\pd}[2]{\frac{\partial #1}{\partial #2}}
\newcommand{\abs}[1]{\left|#1\right|}

\lstdefinelanguage{Julia}%
  {morekeywords={abstract,break,case,catch,const,continue,do,else,elseif,%
      end,export,false,for,function,immutable,import,importall,if,in,%
      macro,module,otherwise,quote,return,switch,true,try,type,typealias,%
      using,while},%
   sensitive=true,%
   alsoother={$},%
   morecomment=[l]\#,%
   morecomment=[n]{\#=}{=\#},%
   morestring=[s]{"}{"},%
   morestring=[m]{'}{'},%
}[keywords,comments,strings]%

\lstset{%
    language         = Julia,
    basicstyle       = \ttfamily,
    keywordstyle     = \bfseries\color{blue},
    stringstyle      = \color{magenta},
    commentstyle     = \color{ForestGreen},
    showstringspaces = false,
}

\begin{document}
\title{\textbf{Final Report}}
\author{Pierce Hunter, Nick Kuckuck, Haoran Wang}
\date{6-07-2020}
\maketitle
\section{1D Approach}
	We solved the 1D equation
	\begin{equation}
		\pd{^2u}{z^2} = -1; \quad 0\leq z\leq 1
	\end{equation}
	with boundary conditions
	\begin{equation}
		\pd{u}{z}\left(1\right) = 0; \quad u(0) = 0
	\end{equation}
	in the four following ways:
	\begin{itemize}
		\item Direct solve on the CPU
		\item CG on the CPU
		\item Direct solve on the GPU
		\item CG on the GPU.
	\end{itemize}
	\section{2D Approach}
	We now seek to expand the problem into 2D and solve using the same techniques. The 2D version of the problem is
	\begin{equation}
		\pd{^2u}{y^2} + \pd{^2u}{z^2} = -1; \quad \begin{dcases}
		0\leq y\leq 1\\
		0\leq z\leq 1
		\end{dcases}
	\end{equation}
	and we expand upon the boundary conditions which become
	\begin{align}
		\pd{u}{y} = 0&\text{ at }y=1\\
		\pd{u}{z} = 0&\text{ at }z=1\\
		u = 0&\text{ at }y=0\vphantom{\pd{u}{y}}\\
		u = 0&\text{ at }z=0\vphantom{\pd{u}{y}}.
	\end{align}
	\subsection{Discretization}
	We discretize in space in both $ y $ and $ z $ using centered difference as
	\begin{equation}
		\frac{u_{i-1,j} - 2u_{i,j} + u_{i+1,j}}{{\Delta y}^2} + \frac{u_{i,j-1} - 2u_{i,j} + u_{i,j+1}}{{\Delta z}^2} = -1
	\end{equation}
	which simplifies when $ \Delta y = \Delta z $ to
	\begin{equation}
		u_{i-1,j} + u_{i,j-1} - 4u_{i,j} + u_{i+1,j} + u_{i,j+1} = -{\Delta y}^2.
	\end{equation}
	This discretization works when $ 2\leq i\leq N $ and $ 2\leq j\leq N $, but we need to solve on the boundaries
	\begin{itemize}
		\item $ i = 2 $
		\begin{itemize}
			\item AND $ j = 2 $
			\begin{align*}
				u_{1,2} + u_{2,1} - 4u_{2,2} + u_{3,2} + u_{2,3} &= -{\Delta y}^2\\
				- 4u_{2,2} + u_{3,2} + u_{2,3} &= -{\Delta y}^2
			\end{align*}
			\item AND $ j = N $
			\begin{align*}
				u_{1,N} + u_{2,N-1} - 4u_{2,N} + u_{3,N} + u_{2,N+1} &= -{\Delta y}^2\\
				u_{2,N-1} - 3u_{2,N} + u_{3,N} &= -{\Delta y}^2
			\end{align*}
			\item OTHERWISE
			\begin{align*}
				u_{1,j} + u_{2,j-1} - 4u_{2,j} + u_{3,j} + u_{2,j+1} &= -{\Delta y}^2\\
				u_{2,j-1} - 4u_{2,j} + u_{3,j} + u_{2,j+1} &= -{\Delta y}^2
			\end{align*}
		\end{itemize}
		\item $ i = N $
		\begin{itemize}
			\item AND $ j = 2 $
			\begin{align*}
				u_{N-1,2} + u_{2,1} - 4u_{N,2} + u_{N+1,2} + u_{N,3} &= -{\Delta y}^2\\
				u_{N-1,2} - 3u_{N,2} + u_{N,3} &= -{\Delta y}^2
			\end{align*}
			\item AND $ j = N $
			\begin{align*}
				u_{N-1,N} + u_{N,N-1} - 4u_{N,N} + u_{N+1,N} + u_{N,N+1} &= -{\Delta y}^2\\
				u_{N-1,N} + u_{N,N-1} - 2u_{N,N} &= -{\Delta y}^2
			\end{align*}
			\item OTHERWISE
			\begin{align*}
				u_{N-1,j} + u_{N,j-1} - 4u_{N,j} + u_{N+1,j} + u_{N,j+1} &= -{\Delta y}^2\\
				u_{N-1,j} + u_{N,j-1} - 3u_{N,j} + u_{N,j+1} &= -{\Delta y}^2
			\end{align*}
		\end{itemize}
		\item $ j = 2 $ AND $ 3\leq i\leq N-1 $
		\begin{align*}
			u_{i-1,2} + u_{i,1} - 4u_{i,2} + u_{i+1,2} + u_{i,3} &= -{\Delta y}^2\\
			u_{i-1,2} - 4u_{i,2} + u_{i+1,2} + u_{i,3} &= -{\Delta y}^2
		\end{align*}
		\item $ j = N $ AND $ 3\leq i\leq N-1 $
		\begin{align*}
			u_{i-1,N} + u_{i,N-1} - 4u_{i,N} + u_{i+1,N} + u_{i,N+1} &= -{\Delta y}^2\\
			u_{i-1,N} + u_{i,N-1} - 3u_{i,N} + u_{i+1,N} &= -{\Delta y}^2
		\end{align*}
	\end{itemize}
	\section{Convert to a Matrix}
	In order to convert this discretization to a matrix that can be used for a direct solve we need to define a new indexing convention. For this we calculate a global index $ k $ as
	\begin{equation}
		k = (i-2)(N-1) + (j-1).
	\end{equation}
	We can then translate our discretization into this new system, starting with the corner (2,2):
	\begin{itemize}
		\item $ (2,2) $
		\begin{align*}
			- 4u_1 + u_{N} + u_2 &= -{\Delta y}^2
		\end{align*}
		\item $ (2,j) $ with $ 3\leq j\leq N-1 $
		\begin{align*}
			u_{j-2} - 4u_{j-1} + u_{N-2+j} + u_j &= -{\Delta y}^2
		\end{align*}
		\item $ (2,N) $
		\begin{align*}
			u_{N-2} - 3u_{N-1} + u_{2N-2} &= -{\Delta y}^2
		\end{align*}
		\item $ (i,2) $ with $ 3\leq i\leq N-1 $
		\begin{align*}
			\begin{split}
				u_{(i-3)(N-1)+1} - 4u_{(i-2)(N-1)+1} \\+ u_{(i-1)(N-1)+1} + u_{(i-2)(N-1)+2} &= -{\Delta y}^2
			\end{split}
		\end{align*}
		\item $ (i,j) $ with $ 3\leq i\leq N-1 $ and $ 3\leq j\leq N-1 $
		\begin{align*}
			\begin{split}
				u_{(i-3)(N-1)+j-1} + u_{(i-2)(N-1)+j-2} - 4u_{(i-2)(N-1)+j-1}\\ + u_{(i-1)(N-1)+j-1} + u_{(i-2)(N-1)+j}& = -{\Delta y}^2
			\end{split}
		\end{align*}
		\item $ (i,N) $ with $ 3\leq i\leq N-1 $
		\begin{align*}
			\begin{split}
				u_{(i-3)(N-1)+N-1} + u_{(i-2)(N-1)+N-2} - 3u_{(i-2)(N-1)+N-1} \\+ u_{(i-1)(N-1)+N-1} &= -{\Delta y}^2
			\end{split}
		\end{align*}
		\item $ (N,2) $
		\begin{align*}
			u_{(N-3)(N-1)+1} - 3u_{(N-2)(N-1)+1} + u_{(N-2)(N-1)+2} &= -{\Delta y}^2
		\end{align*}
		\item $ (N,j) $ with $ 3\leq j\leq N-1 $
		\begin{align*}
			\begin{split}
				u_{(N-3)(N-1)+j-1} + u_{(N-2)(N-1)+j-2} - 3u_{(N-2)(N-1)+j-1}\\ + u_{(N-2)(N-1)+j} &= -{\Delta y}^2
			\end{split}
		\end{align*}
		\item $ (N,N) $
		\begin{align*}
			u_{(N-2)(N-1)} + u_{(N-2)N} - 2u_{(N-1)^2} &= -{\Delta y}^2
		\end{align*}
	\end{itemize}
	So what we end up with is an $ (N-1)^2\times(N-1)^2 $ matrix $ A $ and a solution vector $ b $ with $ (N-1)^2 $ entries. Moving across a row we start at $ (2,2) $, to increase $ j $ by one we move to the right 1 entry, to increase $ i $ by 1 we move the right $ (N-1) $ entries, such that we hit every value of $ j $ first, then move to the next $ i $.
	\newline\indent Along the diagonals of the matrix $ A $ we have $ -4 $ except in the following locations:
	\begin{itemize}
		\item rows $ \alpha(N-1) $ the diagonal entry is $ -3 $ for $ 1\leq \alpha\leq N-2 $
		\item rows $ \left(N-2\right)\left(N-1\right)+\beta $ the diagonal is $ -3 $ for $ 1\leq\beta\leq N-2 $
		\item row $ \left(N-1\right)^2 $ the diagonal is $ -2 $
	\end{itemize}
	We also have 4 other sub-diagonals that will all contain ones except where noted. These represent the following location:
	\begin{itemize}
		\item $ j-1 $ which is directly below the diagonal\\
		In Julia these are the locations: \texttt{[2:(N-1)$^2$, 1:(N-1)$^2$-1]}\\
		Exception: the locations $ (\alpha(N-1) + 1,\alpha(N-1)) $ should be zero for $ 1\leq\alpha\leq N-2 $ 
		\item $ j+1 $ which is directly above the diagonal\\
		In Julia these are the locations: \texttt{[1:(N-1)$^2$-1, 2:(N-1)$^2$]}\\
		Exception: the locations $ (\alpha(N-1),\alpha(N-1)+1) $ should be zero for $ 1\leq\alpha\leq N-2 $ 
		\item $ i-1 $ which are exactly $ N-1 $ below the diagonal\\
		In Julia these are the locations: \texttt{[N:(N-1)$^2$, 1:(N-1)$^2$-(N-1)]}
		\item $ i+1 $ which are exactly $ N+1 $ above the diagonal\\
		In Julia these are the locations: \texttt{[1:(N-1)$^2$-(N-1), N:(N-1)$^2$]}
	\end{itemize}
	Once $ A $ is created it is probably easier to create a column vector of length $ (N-1)^2 $ in which every location contains $ -{\Delta y}^2 $. Once a solution is found via $ u = A\backslash b $ or CG, then $ u $ can be reshaped to the correct dimensions either manually\textemdash \texttt{i = floor((k-1)/(N-1)) + 2}; \texttt{j = mod(k-1,N-1) + 2}\textemdash or via the reshape function transposed\textemdash \texttt{U = reshape(u,N-1,N-1)$'$}. Using reshape without the transpose puts the solution in meshgrid format (with $ y $ as the columns and $ z $ as the rows) similar to looking at a cross-section.\\
	
	\section{Example program run:}
	Direct solve on CPU\\
  0.042633 seconds (8.16 k allocations: 11.199 MiB, 51.33% gc time)\\
norm between our solution and the exact solution =  1.443430e-05 
\\-----------\\

Native Julia CG solve on CPU\\
 15.070843 seconds (34 allocations: 1.985 MiB)\\
norm between our solution and the exact solution =  1.443430e-05 
\\-----------\\

Direct solve on GPU\\
  1.129700 seconds (209 allocations: 9.750 KiB)\\
norm between our solution and the exact solution =  1.443427e-05 
\\-----------\\

CG solve on GPU\\
  3.191565 seconds (4.40 M allocations: 172.127 MiB, 0.92% gc time)\\
norm between our solution and the exact solution =  1.443432e-05 
\\-----------\\

	\section{Code Listing}
	Here is the code listing:
\begin{lstlisting}
using Pkg
Pkg.add("LinearAlgebra")
Pkg.add("SparseArrays")
Pkg.add("IterativeSolvers")
Pkg.add("Printf")
Pkg.add("CuArrays")
Pkg.add("CUDAnative")
Pkg.add("CUDAdrv")

using LinearAlgebra
using SparseArrays
using IterativeSolvers
using Printf

using CuArrays
CuArrays.allowscalar(false)
using CUDAnative
using CUDAdrv

Δz = 5e-5
z = 0:Δz:1
N = length(z)


function exact(z)
    return -1/2 * z.^2 + z
end

# create sparse matrix A
Il = 2:N-1
Jl = 1:N-2
Iu = 1:N-2
Ju = 2:N-1

dl = ones(N-2)
du = ones(N-2)
d = -2*ones(N-1)
A = sparse(Il,Jl,dl,N-1,N-1) + sparse(Iu,Ju,du,N-1,N-1) + sparse(1:N-1,1:N-1,d,N-1,N-1)
A[N-1, N-1] = -1
A .= A / (Δz^2)

b = -ones(N-1, 1)


#   Perform LU solve
println("Direct solve on CPU")
u_dummy_DSCPU = A \ b
@time u_int_DSCPU = A \ b
u_DSCPU = [0; u_int_DSCPU]
# @show umod
@printf "norm between our solution and the exact solution = \x1b[31m %e \x1b[0m\n" sqrt(Δz) * norm(u_DSCPU - exact(z))
println("-----------")
println()

#    Perform CG solve
println("Native Julia CG solve on CPU")
u_dummy_CGCPU = cg(-A, -b)
@time u_int_CGCPU = cg(-A, -b)
u_CGCPU = [0; u_int_CGCPU]
@printf "norm between our solution and the exact solution = \x1b[31m %e \x1b[0m\n" sqrt(Δz) * norm(u_CGCPU - exact(z))

println("-----------")
println()


d_A = CuArray(A)
d_b = CuArray(b)

println("Direct solve on GPU")
u_dummy_DSGPU = d_A \ d_b
@time u_int_DSGPU = d_A \ d_b
u_int_DSGPU_reg = Array(u_int_DSGPU)
u_DSGPU = [0; u_int_DSGPU_reg]
@printf "norm between our solution and the exact solution = \x1b[31m %e \x1b[0m\n" sqrt(Δz) * norm(u_DSGPU - exact(z))
println("-----------")
println()

# CG solve on GPU
d_A = CuArrays.CUSPARSE.CuSparseMatrixCSC(A)
d_b = CuArray(b)
u_cg = CuArray(zeros(size(d_b)))
u_dummy = CuArray(zeros(size(d_b)))

println("CG solve on GPU")
# u_dummy_CGCPU = cg(-d_A, -d_b)
cg!(u_dummy, d_A, d_b)
# @time u_int_CGGPU = cg(-d_A, -d_b)
@time cg!(u_cg, d_A, d_b)
u_int_CGGPU_reg = Array(u_cg)
u_CGGPU = [0; u_int_CGGPU_reg]
@printf "norm between our solution and the exact solution = \x1b[31m %e \x1b[0m\n" sqrt(Δz) * norm(u_CGGPU - exact(z))
println("-----------")
println()
\end{lstlisting}
\end{document}