\documentclass[11pt]{article}

\usepackage{mathtools}
\newcommand{\pd}[2]{\frac{\partial #1}{\partial #2}}

\title{Further Simplified Abstract\\And First Steps}
\author{Pierce Hunter, Nick Kuckuck, Haoran Wang}
\date{22 May 2020}

\begin{document}
	
	\maketitle
	
	\section{Most Simple Version}
	Solve the 1D Poisson's equation to steady-state for a stuck-on glacier
	\begin{equation}
		\pd{^2u}{z^2} = -1; \qquad 0\leq z\leq 1
	\end{equation}
	with the boundary conditions
	\begin{gather}
		u\left(0\right) = 0;\\
		\pd{u}{z}(1) = 0.
	\end{gather}
	We can discretize the domain in space ($ z $) using the standard second-order centered difference approximation
	\begin{equation}
		\pd{^2u_j}{z^2} = \frac{u_{j-1}-2u_j+u_{j+1}}{\left(z_{j+1}-z_j\right)\left(z_j-z_{j-1}\right)} = -1
	\end{equation}
	which, using a consistent distance between nodes, becomes
	\begin{equation}
		\frac{u_{j-1}-2u_j+u_{j+1}}{\Delta z^2} = -1 ~~\text{for}~~ 1\leq j\leq N,
	\end{equation}
	with the boundary conditions
	\begin{gather}
		u_1 = 0;\\
		\pd{u_N}{z} = 0.
	\end{gather}
	For the first equation, when $ j = 2 $, we have
	\begin{equation}
		\frac{u_1 -2u_2 + u_3}{\Delta z^2} = -1 \implies \frac{-2u_2 + u_3}{\Delta z^2} = -1;
	\end{equation}
	and for the final equation when $ j = N $ we have
	\begin{equation}
		\frac{u_{N-1} - 2u_N + u_{N+1}}{\Delta z^2} = -1 ~~\text{with}~~ u_N = u_{N+1} \implies \frac{u_{N-1} - u_N}{\Delta z^2} = -1.
	\end{equation}
	So the system of equations is
	\begin{equation}
		\begin{dcases}
		\frac{-2u_2 + u_3}{\Delta z^2} = -1\\
		\frac{u_{j-1}-2u_j+u_{j+1}}{\Delta z^2} = -1;& 3\leq j\leq N-1\\
		\frac{u_{N-1} - u_N}{\Delta z^2} = -1.
		\end{dcases}
	\end{equation}
	We can represent this system of equations as a matrix ($ A $) of the form
	\begin{equation}
		A = \frac{1}{\Delta z^2}\begin{bmatrix}
		-2&1&0&\cdots&0\\
		1&-2&1&\cdots&0\\
		\vdots&\ddots&\ddots&\ddots&\vdots\\
		0&\cdots&1&-2&1\\
		0&\cdots&0&1&-1
		\end{bmatrix}
	\end{equation}
	with the $ u $-column vector and $ b $-solution vector as
	\begin{equation}
		u = \begin{bmatrix}
		u_2\\
		\vdots\\
		u_N
		\end{bmatrix} \qquad b = \begin{bmatrix}
		-1\\\vdots\\-1
		\end{bmatrix}
	\end{equation}
	such that $ Au = b $.
	
\end{document}